Add proof for entailment laws

src/constr-dot/ConstrLang.v
@@ -13,11 +13,16 @@ Set Implicit Arguments.
 Require Import TLC.LibLN.
 Require Import String.
 
-Require Import Definitions.
+Require Import Definitions RecordAndInertTypes.
+
+
+Inductive tvar : Set :=
+  | tvar_b : nat -> tvar
+  | tvar_f : var -> tvar.
 
 
 Inductive ctyp : Set :=
-  | ctyp_var : avar -> ctyp
+  | ctyp_tvar : tvar -> ctyp
   | ctyp_typ : typ -> ctyp.
 
 
@@ -27,9 +32,267 @@ Inductive constr : Set :=
 | constr_and : constr -> constr -> constr
 | constr_or : constr -> constr -> constr
 | constr_exists_typ : constr -> constr
-| constr_exists_var : constr -> constr
 | constr_sub : ctyp -> ctyp -> constr
-| constr_typ : avar -> ctyp -> constr
+| constr_typ : trm -> ctyp -> constr
 .
 
+(** - true constraint *)
+Notation "⊤" := constr_true.
+
+(** - false constraint *)
+Notation "⊥" := constr_false.
+
+(** - and constraint *)
+Notation "C '⋏' D" := (constr_and C D) (at level 30).
+
+(** - or constraint *)
+Notation "C '⋎' D" := (constr_or C D) (at level 30).
+
+(** - type existence constraint *)
+Notation "'∃t' C" := (constr_exists_typ C) (at level 30).
+
+Notation "x '⦂' T" := (constr_typ x T) (at level 29).
+
+Notation "S '<⦂' T" := (constr_sub S T) (at level 29).
+
+Definition open_rec_tvar (k : nat) (u : var) (tv : tvar) : tvar :=
+  match tv with
+  | tvar_b i => If k = i then tvar_f u else tvar_b i
+  | tvar_f x => tvar_f x
+  end.
+
+
+Definition open_rec_ctyp (k : nat) (u : var) (T : ctyp) : ctyp :=
+  match T with
+  | ctyp_tvar tv => ctyp_tvar (open_rec_tvar k u tv)
+  | ctyp_typ T0 => ctyp_typ T0
+  end.
+
+Fixpoint open_rec_constr (k : nat) (u : var) (C : constr) : constr :=
+  match C with
+  | constr_true => constr_true
+  | constr_false => constr_false
+  | constr_and C1 C2 => constr_and (open_rec_constr k u C1) (open_rec_constr k u C2)
+  | constr_or C1 C2 => constr_or (open_rec_constr k u C1) (open_rec_constr k u C2)
+  | constr_exists_typ C => constr_exists_typ (open_rec_constr (S k) u C)
+  | constr_sub T1 T2 => constr_sub (open_rec_ctyp k u T1) (open_rec_ctyp k u T2)
+  | constr_typ t T => constr_typ t (open_rec_ctyp k u T)
+  end.
+
+
+Definition open_tvar (u : var) (tv : tvar) : tvar := open_rec_tvar 0 u tv.
+Definition open_ctyp (u : var) (T : ctyp) : ctyp := open_rec_ctyp 0 u T.
+Definition open_constr (u : var) (C : constr) : constr := open_rec_constr 0 u C.
+
+
+Fixpoint fv_tvar (tv : tvar) :=
+  match tv with
+  | tvar_b i => \{}
+  | tvar_f x => \{x}
+  end.
+
+
+Fixpoint fv_ctyp (T : ctyp) :=
+  match T with
+  | ctyp_tvar tv => fv_tvar tv
+  | ctyp_typ T => \{}
+  end.
+
+
+Inductive ctyp_lc : ctyp -> Prop :=
+
+| ctyp_typ_lc : forall T, ctyp_lc (ctyp_typ T)
+
+| ctyp_tvar_f_lc : forall x, ctyp_lc (ctyp_tvar (tvar_f x))
+
+.
+
+
+Inductive constr_lc : constr -> Prop :=
+
+| constr_true_lc: constr_lc ⊤
+
+| constr_false_lc: constr_lc ⊥
+
+| constr_and_lc : forall C1 C2,
+    constr_lc C1 ->
+    constr_lc C2 ->
+    constr_lc (C1 ⋏ C2)
+
+| constr_or_lc : forall C1 C2,
+    constr_lc C1 ->
+    constr_lc C2 ->
+    constr_lc (C1 ⋎ C2)
+
+| constr_exists_typ_lc : forall L C,
+    (forall x, x \notin L -> constr_lc (open_constr x C)) ->
+    constr_lc (∃t C)
+
+| constr_sub_lc : forall S T,
+    ctyp_lc S ->
+    ctyp_lc T ->
+    constr_lc (S <⦂ T)
+
+| constr_typ_lc : forall t T,
+    ctyp_lc T ->
+    constr_lc (t ⦂ T)
+
+.
+
+Lemma lc_ctyp_open_unchanged : forall u T,
+    ctyp_lc T ->
+    open_ctyp u T = T.
+Proof.
+  introv Hc.
+  induction Hc; eauto.
+Qed.
+
+Definition tmap := env typ.
+
+Inductive map_ctyp : tmap -> ctyp -> typ -> Prop :=
+
+  | map_ctyp_tvar : forall tm a T,
+      binds a T tm ->
+      map_ctyp tm (ctyp_tvar (tvar_f a)) T
+
+  | map_ctyp_typ : forall tm T,
+      map_ctyp tm (ctyp_typ T) T
+
+.
+
+Lemma map_bound_tvar : forall tm x T T',
+    binds x T tm ->
+    map_ctyp tm (ctyp_tvar (tvar_f x)) T' ->
+    T = T'.
+Proof.
+  introv Hb Hm. inversion Hm; subst.
+  eapply binds_functional.
+  - apply Hb.
+  - apply H1.
+Qed.
+
+
+Lemma map_ctyp_fresh_extend : forall tm X T S S',
+    map_ctyp tm S S' ->
+    X \notin fv_ctyp S ->
+    map_ctyp (tm & X ~ T) S S'.
+Proof.
+  introv Hm Hn.
+  inversion Hm; subst.
+  - apply* map_ctyp_tvar.
+
+
+Inductive satisfy_constr : tmap -> ctx -> constr -> Prop :=
+
+| sat_true : forall tm G,
+    satisfy_constr tm G constr_true
+
+| sat_and : forall tm G C1 C2,
+    satisfy_constr tm G C1 ->
+    satisfy_constr tm G C2 ->
+    satisfy_constr tm G (C1 ⋏ C2)
+
+| sat_or1 : forall tm G C1 C2,
+    satisfy_constr tm G C1 ->
+    satisfy_constr tm G (C1 ⋎ C2)
+
+| sat_or2 : forall tm G C1 C2,
+    satisfy_constr tm G C2 ->
+    satisfy_constr tm G (C1 ⋎ C2)
+
+| sat_exists_typ : forall tm G T L C,
+    (forall X, X \notin L ->
+      satisfy_constr (tm & X ~ T) G (open_constr X C)) ->
+    satisfy_constr tm G (∃t C)
+
+| sat_typ : forall tm G t T T',
+    map_ctyp tm T T' ->
+    G ⊢ t : T' ->
+    satisfy_constr tm G (t ⦂ T)
+
+| sat_sub : forall tm G S S' T T',
+    map_ctyp tm S S' ->
+    map_ctyp tm T T' ->
+    G ⊢ S' <: T' ->
+    satisfy_constr tm G (constr_sub S T)
+
+.
+
+Hint Constructors satisfy_constr constr.
+
+Definition constr_entail (C1 C2 : constr) :=
+  forall tm G,
+    inert G ->
+    satisfy_constr tm G C1 -> satisfy_constr tm G C2.
+
+
+Notation "C '⊩' D" := (constr_entail C D) (at level 50).
+
+Ltac introe := introv H0 H.
+
+Theorem ent_absurd : forall C,
+    ⊥ ⊩ C.
+Proof.
+  introe. inversion H.
+Qed.
+
+
+Theorem ent_tautology : forall C,
+    C ⊩ ⊤.
+Proof. introe. eauto. Qed.
+
+Theorem ent_trans : forall C1 C2 C3,
+    C1 ⊩ C2 ->
+    C2 ⊩ C3 ->
+    C1 ⊩ C3.
+Proof.
+  introv H12 H23.
+  introe.
+  eauto.
+Qed.
+
+Theorem ent_cong_and : forall C C' D,
+    C ⊩ C' ->
+    C ⋏ D ⊩ C' ⋏ D.
+Proof.
+  introv He. introe. inversion H; subst.
+  eauto.
+Qed.
+
+Theorem ent_and_left : forall C D,
+    C ⋏ D ⊩ C.
+Proof. introe. inversion H; subst. eauto. Qed.
+
+Definition ctyp_b (i : nat) := ctyp_tvar (tvar_b i).
+
+(** ∃ U. (S <: U ⋏ U <: T) ⊩ S <: T *)
+Theorem ent_sub_trans : forall S T,
+    ctyp_lc S -> ctyp_lc T ->
+    ∃t (S <⦂ (ctyp_b 0) ⋏ (ctyp_b 0) <⦂ T) ⊩ S <⦂ T.
+Proof.
+  introv Hs Ht.
+  introe. inversion H; subst.
+  unfold open_constr in H4. simpl in H4.
+  case_if. clear C.
+  pick_fresh_gen (L \u fv_ctyp S \u fv_ctyp T) X.
+  specialize (H4 X). assert (X \notin L) as Hnl. { eauto. }
+  specialize (H4 Hnl).
+  inversion H4; subst.
+  pose proof (lc_ctyp_open_unchanged X Hs) as Hsu.
+  unfold open_ctyp in Hsu. rewrite -> Hsu in H6.
+  pose proof (lc_ctyp_open_unchanged X Ht) as Hst.
+  unfold open_ctyp in Hst. rewrite -> Hst in H7.
+  inversion H6; subst.
+  inversion H7; subst.
+  assert (T0 = T') as Heq1.
+  {
+    apply* map_bound_tvar.
+  }
+  assert (T0 = S'0) as Heq2.
+  {
+    apply* map_bound_tvar.
+  }
+  subst.
+  apply sat_sub with (S' := S') (T' := T'0).
+  - 
 
